ccomp-simd/x86/Machregs2.v
@@ -1,0 +1,571 @@
+(* *********************************************************************)
+(*                                                                     *)
+(*              The Compcert verified compiler                         *)
+(*                                                                     *)
+(*          Xavier Leroy, INRIA Paris-Rocquencourt                     *)
+(*                                                                     *)
+(*  Copyright Institut National de Recherche en Informatique et en     *)
+(*  Automatique.  All rights reserved.  This file is distributed       *)
+(*  under the terms of the INRIA Non-Commercial License Agreement.     *)
+(*                                                                     *)
+(* *********************************************************************)
+
+Require Import String.
+Require Import Coqlib.
+Require Import Decidableplus.
+Require Import Maps.
+Require Import AST.
+Require Import Integers.
+Require Import Op.
+
+Require Import mathcomp.ssreflect.ssreflect.
+Require Import mathcomp.ssreflect.ssrbool.
+Require Import mathcomp.ssreflect.eqtype.
+Require Import zint.
+
+
+(** ** Machine registers *)
+
+(** The following type defines the machine registers that can be referenced
+  as locations.  These include:
+- Integer registers that can be allocated to RTL pseudo-registers.
+- Floating-point registers that can be allocated to RTL pseudo-registers.
+- SIMD registers that can be allocated to RTL pseudo-registers.
+- The special [FP0] register denoting the top of the X87 float stack.
+
+  The type [mreg] does not include special-purpose or reserved
+  machine registers such as the stack pointer and the condition codes. *)
+
+Inductive mreg_bank: Type := RI | RF | RX | RY | FP.
+
+Definition mreg_bank_eq (b1 b2: mreg_bank) : bool :=
+ match b1, b2 with
+ | RI, RI | RF, RF | RX, RX | RY, RY | FP, FP => true
+ | _, _ => false
+ end.
+
+Lemma mreg_bank_eqP : Equality.axiom mreg_bank_eq.
+Proof. by move=> b1 b2; apply: (iffP  idP)=>[|<-]; destruct b1, b2. Qed.
+
+Canonical Structure mreg_bank_eqMixin := EqMixin mreg_bank_eqP.
+Canonical Structure mreg_bank_eqType := Eval hnf in @EqType mreg_bank mreg_bank_eqMixin.
+
+Definition mreg_bank_size (rb: mreg_bank) : positive :=
+ match rb with
+ | RI => 15
+ | RF => 16
+ | RX => 16
+ | RY => 16
+ | FP => 1
+ end.
+
+Definition mreg_name := (mreg_bank * eqp_eqType)%type.
+
+Definition mreg_ax rname :=
+ BinPosDef.Pos.leb (snd rname) (mreg_bank_size (fst rname)).
+
+Record mreg := { ridx :> mreg_name ; rbnd : mreg_ax ridx }.
+
+Lemma mregP (r: mreg): mreg_ax (ridx r).
+Proof. by destruct r. Qed.
+
+Definition mreg_eqb (r1 r2: mreg) := ridx r1 == ridx r2.
+
+Lemma mreg_eqb_refl r: mreg_eqb r r.
+Proof. by move: r => [[? ?] ?]; rewrite /mreg_eqb /=. Qed.
+
+Lemma mreg_eqP : Equality.axiom mreg_eqb.
+Proof.
+move=> r1 r2; apply: (iffP  idP) =>[|<-].
+ destruct r1, r2; unfold mreg_eqb => /= /eqP E.
+ move: rbnd0; rewrite E => rbnd0.
+ by have ->: rbnd0 = rbnd1 by apply bool_irrelevance.
+by apply mreg_eqb_refl.
+Qed.
+
+Canonical Structure mreg_eqMixin := EqMixin mreg_eqP.
+Canonical Structure mreg_eqType := Eval hnf in @EqType mreg mreg_eqMixin.
+
+Definition mreg_eq: forall (r1 r2: mreg), {r1 = r2} + {r1 <> r2}.
+Proof.
+move=> r1 r2.
+case E: (mreg_eqb r1 r2).
+ rewrite (eqP E); left; reflexivity.
+right => H.
+by move: E; rewrite H; rewrite mreg_eqb_refl.
+Defined.
+Global Opaque mreg_eq.
+
+Notation machreg rname := {| ridx := rname; rbnd := Logic.eq_refl _ |}.
+
+(** Non-allocatable Special float reg *)
+Notation FP0 := (FP, 1%positive).
+Definition FP0reg : mreg := (machreg FP0).
+
+(** Allocatable integer regs *)
+Notation AX := (RI, 1%positive).
+Definition AXreg := (machreg AX).
+Notation BX := (RI, 2%positive).
+Definition BXreg := (machreg BX).
+Notation CX := (RI, 3%positive).
+Definition CXreg := (machreg CX).
+Notation DX := (RI, 4%positive).
+Definition DXreg := (machreg DX).
+Notation SI := (RI, 5%positive).
+Definition SIreg := (machreg SI).
+Notation DI := (RI, 6%positive).
+Definition DIreg := (machreg DI).
+Notation BP := (RI, 7%positive).
+Definition BPreg := (machreg BP).
+(**r only in 64-bit mode *)
+Notation R8 := (RI, 8%positive).
+Definition R8reg := (machreg R8).
+Notation R9 := (RI, 9%positive).
+Definition R9reg := (machreg R9).
+Notation R10 := (RI, 10%positive).
+Definition R10reg := (machreg R10).
+Notation R11 := (RI, 11%positive).
+Definition R11reg := (machreg R11).
+Notation R12 := (RI, 12%positive).
+Definition R12reg := (machreg R12).
+Notation R13 := (RI, 13%positive).
+Definition R13reg := (machreg R13).
+Notation R14 := (RI, 14%positive).
+Definition R14reg := (machreg R14).
+Notation R15 := (RI, 15%positive).
+Definition R15reg := (machreg R15).
+
+(** Allocatable float regs *)
+Notation F0 := (RF, 1%positive).
+Definition F0reg := (machreg F0).
+Notation F1 := (RF, 2%positive).
+Definition F1reg := (machreg F1).
+Notation F2 := (RF, 3%positive).
+Definition F2reg := (machreg F2).
+Notation F3 := (RF, 4%positive).
+Definition F3reg := (machreg F3).
+Notation F4 := (RF, 5%positive).
+Definition F4reg := (machreg F4).
+Notation F5 := (RF, 6%positive).
+Definition F5reg := (machreg F5).
+Notation F6 := (RF, 7%positive).
+Definition F6reg := (machreg F6).
+Notation F7 := (RF, 8%positive).
+Definition F7reg := (machreg F7).
+(**r only in 64-bit mode *)
+Notation F8 := (RF, 9%positive).
+Definition F8reg := (machreg F8).
+Notation F9 := (RF, 10%positive).
+Definition F9reg := (machreg F9).
+Notation F10 := (RF, 11%positive).
+Definition F10reg := (machreg F10).
+Notation F11 := (RF, 12%positive).
+Definition F11reg := (machreg F11).
+Notation F12 := (RF, 13%positive).
+Definition F12reg := (machreg F12).
+Notation F13 := (RF, 14%positive).
+Definition F13reg := (machreg F13).
+Notation F14 := (RF, 15%positive).
+Definition F14reg := (machreg F14).
+Notation F15 := (RF, 16%positive).
+Definition F15reg := (machreg F15).
+
+(** Allocatable SSE/AVX XMM regs *)
+Notation X0 := (RX, 1%positive).
+Definition X0reg := (machreg X0).
+Notation X1 := (RX, 2%positive).
+Definition X1reg := (machreg X1).
+Notation X2 := (RX, 3%positive).
+Definition X2reg := (machreg X2).
+Notation X3 := (RX, 4%positive).
+Definition X3reg := (machreg X3).
+Notation X4 := (RX, 5%positive).
+Definition X4reg := (machreg X4).
+Notation X5 := (RX, 6%positive).
+Definition X5reg := (machreg X5).
+Notation X6 := (RX, 7%positive).
+Definition X6reg := (machreg X6).
+Notation X7 := (RX, 8%positive).
+Definition X7reg := (machreg X7).
+(**r only in 64-bit mode *)
+Notation X8 := (RX, 9%positive).
+Definition X8reg := (machreg X8).
+Notation X9 := (RX, 10%positive).
+Definition X9reg := (machreg X9).
+Notation X10 := (RX, 11%positive).
+Definition X10reg := (machreg X10).
+Notation X11 := (RX, 12%positive).
+Definition X11reg := (machreg X11).
+Notation X12 := (RX, 13%positive).
+Definition X12reg := (machreg X12).
+Notation X13 := (RX, 14%positive).
+Definition X13reg := (machreg X13).
+Notation X14 := (RX, 15%positive).
+Definition X14reg := (machreg X14).
+Notation X15 := (RX, 16%positive).
+Definition X15reg := (machreg X15).
+
+(** Allocatable AVX2 YMM regs *)
+Notation Y0 := (RY, 1%positive).
+Definition Y0reg := (machreg X0).
+Notation Y1 := (RY, 2%positive).
+Definition Y1reg := (machreg X1).
+Notation Y2 := (RY, 3%positive).
+Definition Y2reg := (machreg X2).
+Notation Y3 := (RY, 4%positive).
+Definition Y3reg := (machreg X3).
+Notation Y4 := (RY, 5%positive).
+Definition Y4reg := (machreg X4).
+Notation Y5 := (RY, 6%positive).
+Definition Y5reg := (machreg X5).
+Notation Y6 := (RY, 7%positive).
+Definition Y6reg := (machreg X6).
+Notation Y7 := (RY, 8%positive).
+Definition Y7reg := (machreg X7).
+Notation Y8 := (RY, 9%positive).
+Definition Y8reg := (machreg Y8).
+Notation Y9 := (RY, 10%positive).
+Definition Y9reg := (machreg Y9).
+Notation Y10 := (RY, 11%positive).
+Definition Y10reg := (machreg Y10).
+Notation Y11 := (RY, 12%positive).
+Definition Y11reg := (machreg Y11).
+Notation Y12 := (RY, 13%positive).
+Definition Y12reg := (machreg Y12).
+Notation Y13 := (RY, 14%positive).
+Definition Y13reg := (machreg Y13).
+Notation Y14 := (RY, 15%positive).
+Definition Y14reg := (machreg Y14).
+Notation Y15 := (RY, 16%positive).
+Definition Y15reg := (machreg Y15).
+
+Print Pos.iter.
+
+Definition all_mregs : list mreg :=
+     AXreg :: BXreg :: CXreg :: DXreg :: SIreg :: DIreg :: BPreg
+  :: R8reg :: R9reg :: R10reg :: R11reg :: R12reg :: R13reg :: R14reg :: R15reg
+  :: F0reg :: F1reg :: F2reg :: F3reg :: F4reg :: F5reg :: F6reg :: F7reg
+  :: F8reg :: F9reg :: F10reg :: F11reg :: F12reg :: F13reg :: F14reg :: F15reg
+  :: X0reg :: X1reg :: X2reg :: X3reg :: X4reg :: X5reg :: X6reg :: X7reg
+  :: X8reg :: X9reg :: X10reg :: X11reg :: X12reg :: X13reg :: X14reg :: X15reg
+  :: Y0reg :: Y1reg :: Y2reg :: Y3reg :: Y4reg :: Y5reg :: Y6reg :: Y7reg
+  :: Y8reg :: Y9reg :: Y10reg :: Y11reg :: Y12reg :: Y13reg :: Y14reg :: Y15reg
+  :: FP0reg :: nil.
+
+Lemma all_mregs_complete:
+  forall (r: mreg), In r all_mregs.
+Proof.
+  assert (forall r, proj_sumbool (In_dec mreg_eq r all_mregs) = true).
+   admit.
+  intros. specialize (H r). InvBooleans. auto.
+Admitted.
+
+Instance Decidable_eq_mreg : forall (x y: mreg), Decidable (eq x y) := Decidable_eq mreg_eq.
+
+Instance Finite_mreg : Finite mreg := {
+  Finite_elements := all_mregs;
+  Finite_elements_spec := all_mregs_complete
+}.
+
+Definition mreg_type (r: mreg): typ :=
+  match r with
+  | AX | BX | CX | DX | SI | DI | BP => if Archi.ptr64 then Tany64 else Tany32
+  | R8 | R9 | R10 | R11 | R12 | R13 | R14 | R15 => Tany64
+  | X0 | X1 | X2 | X3 | X4 | X5 | X6 | X7 => Tany64
+  | X8 | X9 | X10 | X11 | X12 | X13 | X14 | X15 => Tany64
+  | FP0 => Tany64
+  end.
+
+Local Open Scope positive_scope.
+
+Module IndexedMreg <: INDEXED_TYPE.
+  Definition t := mreg.
+  Definition eq := mreg_eq.
+  Definition index (r: mreg): positive :=
+    match r with
+    | AX => 1 | BX => 2 | CX => 3 | DX => 4 | SI => 5 | DI => 6 | BP => 7
+    | R8 => 8 | R9 => 9 | R10 => 10 | R11 => 11 | R12 => 12 | R13 => 13 | R14 => 14 | R15 => 15
+    | X0 => 16 | X1 => 17 | X2 => 18 | X3 => 19 | X4 => 20 | X5 => 21 | X6 => 22 | X7 => 23
+    | X8 => 24 | X9 => 25 | X10 => 26 | X11 => 27 | X12 => 28 | X13 => 29 | X14 => 30 | X15 => 31
+    | FP0 => 32
+    end.
+  Lemma index_inj:
+    forall r1 r2, index r1 = index r2 -> r1 = r2.
+  Proof.
+    decide_goal.
+  Qed.
+End IndexedMreg.
+
+Definition is_stack_reg (r: mreg) : bool :=
+  match r with FP0 => true | _ => false end.
+
+(** ** Names of registers *)
+
+Local Open Scope string_scope.
+
+Definition register_names :=
+  ("RAX", AX) :: ("RBX", BX) :: ("RCX", CX) :: ("RDX", DX) ::
+  ("RSI", SI) :: ("RDI", DI) :: ("RBP", BP) ::
+  ("EAX", AX) :: ("EBX", BX) :: ("ECX", CX) :: ("EDX", DX) ::
+  ("ESI", SI) :: ("EDI", DI) :: ("EBP", BP) ::
+  ("R8", R8) :: ("R9", R9) :: ("R10", R10) :: ("R11", R11) ::
+  ("R12", R12) :: ("R13", R13) :: ("R14", R14) :: ("R15", R15) ::
+  ("XMM0", X0) :: ("XMM1", X1) :: ("XMM2", X2) :: ("XMM3", X3) ::
+  ("XMM4", X4) :: ("XMM5", X5) :: ("XMM6", X6) :: ("XMM7", X7) ::
+  ("XMM8", X8) :: ("XMM9", X9) :: ("XMM10", X10) :: ("XMM11", X11) ::
+  ("XMM12", X12) :: ("XMM13", X13) :: ("XMM14", X14) :: ("XMM15", X15) ::
+  ("ST0", FP0) :: nil.
+ 
+Definition register_by_name (s: string) : option mreg :=
+  let fix assoc (l: list (string * mreg)) : option mreg :=
+    match l with
+    | nil => None
+    | (s1, r1) :: l' => if string_dec s s1 then Some r1 else assoc l'
+    end
+  in assoc register_names.
+
+(** ** Destroyed registers, preferred registers *)
+
+Definition destroyed_by_op (op: operation): list mreg :=
+  match op with
+  | Ocast8signed | Ocast8unsigned => AX :: nil
+  | Omulhs => AX :: DX :: nil
+  | Omulhu => AX :: DX :: nil
+  | Odiv => AX :: DX :: nil
+  | Odivu => AX :: DX :: nil
+  | Omod => AX :: DX :: nil
+  | Omodu => AX :: DX :: nil
+  | Oshrximm _ => CX :: nil
+  | Omullhs => AX :: DX :: nil
+  | Omullhu => AX :: DX :: nil
+  | Odivl => AX :: DX :: nil
+  | Odivlu => AX :: DX :: nil
+  | Omodl => AX :: DX :: nil
+  | Omodlu => AX :: DX :: nil
+  | Oshrxlimm _ => DX :: nil
+  | Ocmp _ => AX :: CX :: nil
+  | _ => nil
+  end.
+
+Definition destroyed_by_load (chunk: memory_chunk) (addr: addressing): list mreg :=
+  nil.
+
+Definition destroyed_by_store (chunk: memory_chunk) (addr: addressing): list mreg :=
+  match chunk with
+  | Mint8signed | Mint8unsigned => if Archi.ptr64 then nil else AX :: CX :: nil
+  | _ => nil
+  end.
+
+Definition destroyed_by_cond (cond: condition): list mreg :=
+  nil.
+
+Definition destroyed_by_jumptable: list mreg :=
+  AX :: DX :: nil.
+
+Fixpoint destroyed_by_clobber (cl: list string): list mreg :=
+  match cl with
+  | nil => nil
+  | c1 :: cl =>
+      match register_by_name c1 with
+      | Some r => r :: destroyed_by_clobber cl
+      | None   => destroyed_by_clobber cl
+      end
+  end.
+
+Definition destroyed_by_builtin (ef: external_function): list mreg :=
+  match ef with
+  | EF_memcpy sz al =>
+      if zle sz 32 then CX :: X7 :: nil else CX :: SI :: DI :: nil
+  | EF_vstore (Mint8unsigned|Mint8signed) =>
+      if Archi.ptr64 then nil else AX :: CX :: nil
+  | EF_builtin name sg =>
+      if string_dec name "__builtin_va_start" then AX :: nil
+      else if string_dec name "__builtin_write16_reversed"
+           || string_dec name "__builtin_write32_reversed"
+      then CX :: DX :: nil
+      else nil
+  | EF_inline_asm txt sg clob => destroyed_by_clobber clob
+  | _ => nil
+  end.
+
+Definition destroyed_at_function_entry: list mreg :=
+  (* must include [destroyed_by_setstack ty] *)
+  AX :: FP0 :: nil.
+
+Definition destroyed_by_setstack (ty: typ): list mreg :=
+  match ty with
+  | Tfloat | Tsingle => FP0 :: nil
+  | _ => nil
+  end.
+
+Definition destroyed_at_indirect_call: list mreg :=
+  AX :: nil.
+
+Definition temp_for_parent_frame: mreg :=
+  AX.
+
+Definition mregs_for_operation (op: operation): list (option mreg) * option mreg :=
+  match op with
+  | Omulhs => (Some AX :: None :: nil, Some DX)
+  | Omulhu => (Some AX :: None :: nil, Some DX)
+  | Odiv => (Some AX :: Some CX :: nil, Some AX)
+  | Odivu => (Some AX :: Some CX :: nil, Some AX)
+  | Omod => (Some AX :: Some CX :: nil, Some DX)
+  | Omodu => (Some AX :: Some CX :: nil, Some DX)
+  | Oshl => (None :: Some CX :: nil, None)
+  | Oshr => (None :: Some CX :: nil, None)
+  | Oshru => (None :: Some CX :: nil, None)
+  | Oshrximm _ => (Some AX :: nil, Some AX)
+  | Omullhs => (Some AX :: None :: nil, Some DX)
+  | Omullhu => (Some AX :: None :: nil, Some DX)
+  | Odivl => (Some AX :: Some CX :: nil, Some AX)
+  | Odivlu => (Some AX :: Some CX :: nil, Some AX)
+  | Omodl => (Some AX :: Some CX :: nil, Some DX)
+  | Omodlu => (Some AX :: Some CX :: nil, Some DX)
+  | Oshll => (None :: Some CX :: nil, None)
+  | Oshrl => (None :: Some CX :: nil, None)
+  | Oshrlu => (None :: Some CX :: nil, None)
+  | Oshrxlimm _ => (Some AX :: nil, Some AX)
+  | _ => (nil, None)
+  end.
+
+Definition mregs_for_builtin (ef: external_function): list (option mreg) * list (option mreg) :=
+  match ef with
+  | EF_memcpy sz al =>
+     if zle sz 32 then (Some AX :: Some DX :: nil, nil) else (Some DI :: Some SI :: nil, nil)
+  | EF_builtin name sg =>
+     if string_dec name "__builtin_negl" then
+       (Some DX :: Some AX :: nil, Some DX :: Some AX :: nil)
+     else if string_dec name "__builtin_addl"
+          || string_dec name "__builtin_subl" then
+       (Some DX :: Some AX :: Some CX :: Some BX :: nil, Some DX :: Some AX :: nil)
+     else if string_dec name "__builtin_mull" then
+       (Some AX :: Some DX :: nil, Some DX :: Some AX :: nil)
+     else if string_dec name "__builtin_va_start" then
+       (Some DX :: nil, nil)
+     else if (negb Archi.ptr64) && string_dec name "__builtin_bswap64" then
+       (Some AX :: Some DX :: nil, Some DX :: Some AX :: nil)
+     else
+       (nil, nil)
+  | _ => (nil, nil)
+  end.
+
+Global Opaque
+    destroyed_by_op destroyed_by_load destroyed_by_store
+    destroyed_by_cond destroyed_by_jumptable destroyed_by_builtin
+    destroyed_by_setstack destroyed_at_function_entry temp_for_parent_frame
+    mregs_for_operation mregs_for_builtin.
+
+(** Two-address operations.  Return [true] if the first argument and
+  the result must be in the same location *and* are unconstrained
+  by [mregs_for_operation]. *)
+
+Definition two_address_op (op: operation) : bool :=
+  match op with
+  | Omove => false
+  | Ointconst _ => false
+  | Olongconst _ => false
+  | Ofloatconst _ => false
+  | Osingleconst _ => false
+  | Oindirectsymbol _ => false
+  | Ocast8signed => false
+  | Ocast8unsigned => false
+  | Ocast16signed => false
+  | Ocast16unsigned => false
+  | Oneg => true
+  | Osub => true
+  | Omul => true
+  | Omulimm _ => true
+  | Omulhs => false
+  | Omulhu => false
+  | Odiv => false
+  | Odivu => false
+  | Omod => false
+  | Omodu => false
+  | Oand => true
+  | Oandimm _ => true
+  | Oor => true
+  | Oorimm _ => true
+  | Oxor => true
+  | Oxorimm _ => true
+  | Onot => true
+  | Oshl => true
+  | Oshlimm _ => true
+  | Oshr => true
+  | Oshrimm _ => true
+  | Oshrximm _ => false
+  | Oshru => true
+  | Oshruimm _ => true
+  | Ororimm _ => true
+  | Oshldimm _ => true
+  | Olea addr => false
+  | Omakelong => true
+  | Olowlong => true
+  | Ohighlong => true
+  | Ocast32signed => false
+  | Ocast32unsigned => false
+  | Onegl => true
+  | Oaddlimm _ => true
+  | Osubl => true
+  | Omull => true
+  | Omullimm _ => true
+  | Omullhs => false
+  | Omullhu => false
+  | Odivl => false
+  | Odivlu => false
+  | Omodl => false
+  | Omodlu => false
+  | Oandl => true
+  | Oandlimm _ => true
+  | Oorl => true
+  | Oorlimm _ => true
+  | Oxorl => true
+  | Oxorlimm _ => true
+  | Onotl => true
+  | Oshll => true
+  | Oshllimm _ => true
+  | Oshrl => true
+  | Oshrlimm _ => true
+  | Oshrxlimm _ => false
+  | Oshrlu => true
+  | Oshrluimm _ => true
+  | Ororlimm _ => true
+  | Oleal addr => false
+  | Onegf => true
+  | Oabsf => true
+  | Oaddf => true
+  | Osubf => true
+  | Omulf => true
+  | Odivf => true
+  | Onegfs => true
+  | Oabsfs => true
+  | Oaddfs => true
+  | Osubfs => true
+  | Omulfs => true
+  | Odivfs => true
+  | Osingleoffloat => false
+  | Ofloatofsingle => false
+  | Ointoffloat => false
+  | Ofloatofint => false
+  | Ointofsingle => false
+  | Osingleofint => false
+  | Olongoffloat => false
+  | Ofloatoflong => false
+  | Olongofsingle => false
+  | Osingleoflong => false
+  | Ocmp c => false
+  | Osel c op => true
+  end.
+
+(* Constraints on constant propagation for builtins *)
+
+Definition builtin_constraints (ef: external_function) :
+                                       list builtin_arg_constraint :=
+  match ef with
+  | EF_vload _ => OK_addressing :: nil
+  | EF_vstore _ => OK_addressing :: OK_default :: nil
+  | EF_memcpy _ _ => OK_addrstack :: OK_addrstack :: nil
+  | EF_annot kind txt targs => map (fun _ => OK_all) targs
+  | EF_debug kind txt targs => map (fun _ => OK_all) targs
+  | _ => nil
+  end.
